WIP Flag-based effect poly

state/MST.Tot.fst
@@ -7,6 +7,87 @@ open FStar.Monotonic.Heap
 open FStar.Ghost
 include MST.Repr (** just for witnessed **)
 
+(** Flag-based effect polymorphsim **)
+
+type tflag =
+| All
+| None
+
+let rec satisfies #a (t : free a) (f : tflag) =
+  match f with
+  | All -> True
+  | None ->
+    begin match t with
+    | Return x -> True
+    | Read r cont -> False
+    | Write r v cont -> False
+    | Alloc init cont -> False
+    | Witness pred cont -> cont () `satisfies` f
+    | Recall pred cont -> cont () `satisfies` f
+    | PartialCall pre fnc -> forall r. fnc r  `satisfies` f
+    | GetHeap cont -> False
+    end
+
+let (⊕) (flag1:tflag) (flag2:tflag) : tflag =
+  match flag1, flag2 with
+  | None, None -> None
+  | None, fl -> fl
+  | fl, None -> fl
+  | _, _ -> All
+
+let (≼) (flag1:tflag) (flag2:tflag) : Type0 =
+  match flag1, flag2 with
+  | None, _ -> True
+  | All, All -> True
+  | All, _ -> False
+
+let plus_compat_le (f1 f2 : tflag) : Lemma (f1 ≼ (f1⊕f2)) = ()
+let plus_comm      (f1 f2 : tflag) : Lemma (f1⊕f2 == f2⊕f1) = ()
+
+let rec sat_le (f1:tflag) (f2:tflag{f1 ≼ f2}) (m : free 'a) :
+  Lemma (satisfies m f1 ==> satisfies m f2) =
+  match m with
+  | Return _ -> ()
+  | Alloc _ o
+  | Witness _ o
+  | Recall _ o
+  | Read _ o
+  | PartialCall _ o ->
+    Classical.forall_intro
+     ((fun r -> sat_le f1 f2 (o r)) <: r:_ -> Lemma (satisfies (o r) f1 ==> satisfies (o r) f2))
+  | Write r v o -> ()
+  | GetHeap cont -> ()
+
+let rec sat_bind (fl:tflag) (v : free 'a) (f : 'a -> free 'b) :
+  Lemma (
+    v `satisfies` fl /\ (forall x. f x `satisfies` fl) ==>
+    free_bind v f `satisfies` fl
+  )
+= match v with
+  | Return _ -> ()
+  | PartialCall i o
+  | Alloc i o
+  | Witness i o
+  | Recall i o
+  | Read i o ->
+    Classical.forall_intro
+      ((fun r -> sat_bind fl (o r) f) <: r:_ -> Lemma ((o r) `satisfies` fl /\ (forall x. f x `satisfies` fl) ==> free_bind (o r) f `satisfies` fl))
+  | Write r v o -> ()
+  | GetHeap cont -> ()
+
+let sat_bind_add (fl_v fl_f:tflag) (v : free 'a) (f : 'a -> free 'b) :
+  Lemma (
+    v `satisfies` fl_v /\ (forall x. f x `satisfies` fl_f) ==>
+    free_bind v f `satisfies` (fl_v ⊕ fl_f)
+  )
+  =
+  sat_le fl_v (fl_v ⊕ fl_f) v;
+  let aux x : Lemma (f x `satisfies` fl_f ==> f x `satisfies` (fl_v ⊕ fl_f)) =
+    sat_le fl_f (fl_v ⊕ fl_f) (f x)
+  in
+  Classical.forall_intro aux;
+  sat_bind (fl_v ⊕ fl_f) v f
+
 (* Total state effect --- the heap is first-order *)
 
 let st_pre   = st_pre_h   heap
@@ -14,55 +95,66 @@ let st_post' = st_post_h' heap
 let st_post  = st_post_h  heap
 let st_wp    = st_mwp_h   heap
 
-val mheap : (a:Type u#a) -> st_wp a -> Type u#(max 1 a)
-let mheap = mst
+val mheap : (a:Type u#a) -> erased tflag -> st_wp a -> Type u#(max 1 a)
+let mheap a f w = t: mst a w { t `satisfies` f }
 
 val mheap_bind :
   (a : Type u#a) ->
   (b : Type u#b) ->
+  (fv : erased tflag) ->
   (wp_v : st_wp a) ->
+  (ff : erased tflag) ->
   wp_f: (a -> st_wp b) ->
-  (v : mheap a wp_v) ->
-  (f : (x:a -> mheap b (wp_f x))) ->
-  Tot (mheap b (st_bind_wp heap a b wp_v wp_f))
-let mheap_bind a b wp_v wp_f v f = mst_bind #a #b #wp_v #wp_f v f
+  (v : mheap a fv wp_v) ->
+  (f : (x:a -> mheap b ff (wp_f x))) ->
+  Tot (mheap b (fv ⊕ ff) (st_bind_wp heap a b wp_v wp_f))
+let mheap_bind a b ff wp_v fv wp_f v f =
+  sat_bind_add fv ff v f ;
+  mst_bind #a #b #wp_v #wp_f v f
 
-val mheap_return : (a:Type) -> (x:a) -> mheap a (st_return heap a x)
-let mheap_return a = mst_return #a
+let mheap_return (a : Type) (x : a) :
+  mheap a None (st_return heap a x) by (compute ())
+= mst_return x
 
 
 val mheap_subcomp :
   (a : Type u#a) ->
+  (flag1 : erased tflag) ->
   (wp1 : st_wp a) ->
+  (flag2 : erased tflag) ->
   (wp2 : st_wp a) ->
-  (v : mheap a wp1) ->
-  Pure (mheap a wp2) (requires (wp1 ⊑ wp2)) (ensures (fun _ -> True))
-let mheap_subcomp a wp1 wp2 = mst_subcomp #a #wp1 #wp2
+  (v : mheap a flag1 wp1) ->
+  Pure (mheap a flag2 wp2) (requires flag1 ≼ flag2 /\ wp1 ⊑ wp2) (ensures (fun _ -> True))
+let mheap_subcomp a flag1 wp1 flag2 wp2 v =
+  sat_le flag1 flag2 v ;
+  mst_subcomp v
 
 let mheap_if_then_else (a : Type u#a)
+  (flag1 : erased tflag)
   (#wp1 : st_wp a)
+  (flag2 : erased tflag)
   (#wp2 : st_wp a)
-  (f : mheap a wp1) (g : mheap a wp2) (b : bool) : Type =
-  mheap a (st_if_then_else heap a b wp1 wp2)
+  (f : mheap a flag1 wp1) (g : mheap a flag2 wp2) (b : bool) : Type =
+  mheap a (flag1 ⊕ flag2) (st_if_then_else heap a b wp1 wp2)
 
 [@@ top_level_effect]
 total
 reifiable
 reflectable
 effect {
-  STATEwp (a:Type) (wp : st_wp a)
+  STATEwp (a:Type) (flag:erased tflag) (wp : st_wp a)
   with {
-       repr       = mheap
-     ; return     = mheap_return
-     ; bind       = mheap_bind
-     ; subcomp    = mheap_subcomp
-     ; if_then_else = mheap_if_then_else
-     }
+    repr         = mheap ;
+    return       = mheap_return ;
+    bind         = mheap_bind ;
+    subcomp      = mheap_subcomp ;
+    if_then_else = mheap_if_then_else
+  }
 }
 
-effect ST (a:Type) (pre:st_pre) (post: (h:heap -> Tot (st_post' a (pre h)))) =
-  STATEwp a (fun (p:st_post a) (h0:heap) -> pre h0 /\ (forall a h1. h0 `heap_rel` h1 /\ post h0 a h1 ==> p a h1))
-effect St (a:Type) = ST a (fun h -> True) (fun h0 r h1 -> True)
+effect ST (a:Type) (fl:tflag) (pre:st_pre) (post: (h:heap -> Tot (st_post' a (pre h)))) =
+  STATEwp a fl (fun (p:st_post a) (h0:heap) -> pre h0 /\ (forall a h1. h0 `heap_rel` h1 /\ post h0 a h1 ==> p a h1))
+effect St (a:Type) = ST a None (fun h -> True) (fun h0 r h1 -> True)
 
 unfold
 let wp_lift_pure_st (w : pure_wp 'a) : st_wp 'a =
@@ -73,50 +165,50 @@ val lift_pure_mst :
   a: Type u#a ->
   w: pure_wp a ->
   f: (eqtype_as_type unit -> PURE a w) ->
-  Tot (mheap a (wp_lift_pure_st w))
+  Tot (mheap a None (wp_lift_pure_st w))
 let lift_pure_mst a w f =
   FStar.Monotonic.Pure.elim_pure_wp_monotonicity_forall ();
   let lhs = partial_return (as_requires w) in
   let rhs = (fun (pre:(squash (as_requires w))) -> mheap_return a (f pre)) in
-  let m = mheap_bind _ _ _ _ lhs rhs in
-  mheap_subcomp _ _ _ m
+  let m = mheap_bind _ _ None _ _ _ lhs rhs in
+  mheap_subcomp _ _ _ _ _ m
 
 sub_effect PURE ~> STATEwp = lift_pure_mst
 
 let contains_pred (#a:Type) (#rel:preorder a) (r:mref a rel) : heap_predicate_stable =
   fun h -> h `contains` r
 
-let witness (pred:heap_predicate_stable) : STATEwp unit (fun p h -> pred h /\ (witnessed pred ==> p () h)) =
+let witness (pred:heap_predicate_stable) : STATEwp unit All (fun p h -> pred h /\ (witnessed pred ==> p () h)) =
   STATEwp?.reflect (mst_witness pred)
 
-let recall (pred:heap_predicate_stable) : STATEwp unit (fun p h -> witnessed pred /\ (pred h ==> p () h)) =
+let recall (pred:heap_predicate_stable) : STATEwp unit All (fun p h -> witnessed pred /\ (pred h ==> p () h)) =
   STATEwp?.reflect (mst_recall pred)
 
 let alloc (#a:Type) (#rel:preorder a) (init:a) :
-  ST (mref a rel) (fun h -> True) (alloc_post init)
+  ST (mref a rel) All (fun h -> True) (alloc_post init)
 = STATEwp?.reflect (mst_alloc init)
 
 let read (#a:Type) (#rel:preorder a) (r:mref a rel) :
-  STATEwp a (fun p h0 -> h0 `contains` r /\ p (sel h0 r) h0)
+  STATEwp a All (fun p h0 -> h0 `contains` r /\ p (sel h0 r) h0)
 = STATEwp?.reflect (mst_read r)
 
 let write (#a:Type) (#rel:preorder a) (r:mref a rel) (v:a) :
-  ST unit
+  ST unit All
     (fun h0 -> h0 `contains` r /\ rel (sel h0 r) v)
     (write_post #a #rel r v)
 = STATEwp?.reflect (mst_write r v)
 
 let op_Bang (#a:Type) (#rel:preorder a) (r:mref a rel)
-  : STATEwp a (fun p h0 -> h0 `contains` r /\ p (sel h0 r) h0)
+  : STATEwp a All (fun p h0 -> h0 `contains` r /\ p (sel h0 r) h0)
 = read #a #rel r
 
 let op_Colon_Equals (#a:Type) (#rel:preorder a) (r:mref a rel) (v:a)
-  : ST unit
+  : ST unit All
     (fun h0 -> h0 `contains` r /\ rel (sel h0 r) v)
     (write_post r v)
 = write #a #rel r v
 
-let get_heap () : ST (erased heap) (fun h0 -> True) (fun h0 r h1 -> h0 == h1 /\ reveal r == h0) =
+let get_heap () : ST (erased heap) All (fun h0 -> True) (fun h0 r h1 -> h0 == h1 /\ reveal r == h0) =
   STATEwp?.reflect (mst_get_heap)
 
 type ref (a:Type0) = mref a (FStar.Heap.trivial_preorder a)
